Bash Grep - verificado

Part 2 - Dafny/grep-naive/grep.dfy
@@ -7,13 +7,85 @@
 
 include "Io.dfy"
 
+method ArrayFromSeq<T>(s: seq<T>) returns (a: array<T>)
+  ensures |s| == a.Length
+  ensures a[0.. a.Length] == s
+{
+  a := new T[|s|] ( i requires 0 <= i < |s| => s[i] );
+}
+
+method countItem<T(==)>(arr: array<T>, item: T) returns (count: nat) 
+requires arr.Length > 0
+ensures count == countF(arr[0..arr.Length], item)
+{
+  var i := 0;
+  count := 0;
+
+  while (i < arr.Length) 
+  invariant i <= arr.Length && count == countF(arr[0..i], item) 
+  decreases arr.Length - i
+  {
+    if arr[i] == item {
+      count := count + 1;
+    }
+    i := i + 1;
+  }
+}
+
+function countF<T>(items: seq<T>, item: T): nat
+
+{
+  multiset(items)[item]
+}
+
+method splitArrayBy<T(==)>(arr: array<T>, item: T) returns (a: array<array<T>>)
+requires arr.Length > 0
+ensures fresh(a) && a.Length > 0 && a.Length == countF(arr[0..arr.Length], item) + 1
+{
+  var from := 0;
+  var to := 0;
+  var l_cnt := 0;
+  var lines := countItem(arr, item);
+  lines := lines + 1;
+
+  if lines == 0 {
+    return new array<T>[1] (_ => arr);
+  }
+
+  a := new array<T>[lines];
+
+  while(to < arr.Length && from < arr.Length && l_cnt < lines) 
+  decreases arr.Length - to
+  decreases arr.Length - from
+  invariant l_cnt <= lines && to + 1 > from
+  invariant to <= arr.Length && from <= arr.Length
+  invariant a.Length == countF(arr[0..arr.Length], item) + 1
+  {
+    if (arr[to] == item){
+      a[l_cnt] := ArrayFromSeq(arr[from..to + 1]);
+      l_cnt := l_cnt + 1;
+      from := to + 1;
+    }
+    if(l_cnt == lines-1 && to == arr.Length-1 ){
+      var tmp := [];
+      var n := [item];
+      tmp := arr[from..] + n;
+      a[l_cnt] := ArrayFromSeq(tmp);
+      l_cnt := l_cnt + 1;
+    } 
+    to := to + 1;
+  }
+}
+
+
+
 predicate inRange(i: int, len: int, j: int, len2: int) {
   0 <= i < len && 0 <= j < len2
 }
 
-predicate sorted(s: seq<nat>)
+predicate method sorted(s: seq<nat>, diff: nat)
 {
-  forall i,j :: 0 <= i < j < |s| ==> s[i] <= s[j]
+  forall i,j :: 0 <= i < j < |s| ==> s[i] <= s[j] - diff
 }
 
 predicate IndexIsMatch(word: array<char>, query:array<char>, index: nat) 
@@ -33,7 +105,8 @@ requires n <= query.Length
 // se count words de index até index + query.Length
 method IsMatch(word: array<char>, query: array<char>, index: int) returns (m: bool)
 requires 0 <= index <= word.Length - query.Length
-ensures m ==> IndexIsMatch(word, query, index)
+ensures m <==> IndexIsMatch(word, query, index)
+ensures m ==> exists v :: 0 <= v <= word.Length - query.Length && IndexIsMatch(word, query, v)
 {
   //var cnt := CountConsecutiveChars(word[index..index+query.Length], query[..]);
   var j := 0;
@@ -41,7 +114,6 @@ ensures m ==> IndexIsMatch(word, query, index)
   invariant index + j <= word.Length
   invariant j <= query.Length
   invariant IsMatchN(word, query, index, j)
-  //invariant j + 1 == C(word[index..index + j + 1], query[..j + 1])
   {
     j := j + 1;
   }
@@ -53,32 +125,30 @@ method  GrepNaive(word: array<char>, query: array<char>) returns (found: bool, i
 requires word.Length >= query.Length
 requires word.Length > 0
 requires query.Length > 0
-ensures forall k :: 0 <= k < |indexes| ==> indexes[k] < word.Length
-ensures forall k :: 0 <= k < |indexes| ==> indexes[k] + query.Length <= word.Length
-ensures forall k :: 0 <= k < |indexes| ==> IndexIsMatch(word, query, indexes[k])
-
+ensures forall k :: 0 <= k < |indexes| ==> indexes[k] + query.Length <= word.Length && indexes[k] < word.Length && IndexIsMatch(word, query, indexes[k])
+ensures found ==> AnyMatch(word, query)
 {
-  var i := 0;
+  var i, m := 0, false;
   found := false;
   indexes := [];
 
 
   while i <= word.Length - query.Length
-  invariant forall k :: 0 <= k < |indexes| ==> indexes[k] < word.Length
-  invariant forall k :: 0 <= k < |indexes| ==> indexes[k] + query.Length <= word.Length
+  invariant forall k :: 0 <= k < |indexes| ==> 0 <= indexes[k] <= word.Length - query.Length
   invariant forall k :: 0 <= k < |indexes| ==> IndexIsMatch(word, query, indexes[k])
-
-  {
-    //var j := CountWords(word[i..i+query.Length], query[..]);
-    
-    var m := IsMatch(word, query, i);
+  invariant forall k :: 0 <= k < |indexes| ==> 0 <= indexes[k] <= i
+  invariant found ==> AnyMatch(word, query)
+  decreases word.Length - query.Length - i
+  {    
+    m := IsMatch(word, query, i);
 
     if m {
+      found := m;
       indexes := indexes + [i];
     }
+    
     i := i + 1;
   }
-  return |indexes| > 0, indexes;
 }
 
 method CastArray(a: array<byte>) returns (chars: array<char>)
@@ -91,43 +161,40 @@ ensures forall i :: 0 <= i < a.Length ==> a[i] as char == chars[i]
   chars := new char[a.Length] (i requires 0 <= i < a.Length reads a => a[i] as char);
 }
 
-method BashGrep(word: array<char>, query: array<char>) returns (found: bool, rst: seq<char>)
+
+predicate AnyMatch(word: array<char>, query: array<char>) 
+reads word, query
+{
+  exists i :: 0 <= i <= word.Length - query.Length && IndexIsMatch(word, query, i)
+}
+
+method BashGrep(word: array<char>, query: array<char>) returns (found: bool, lines: seq<array<char>>)
 requires word.Length > 0
 requires query.Length > 0
 requires word.Length >= query.Length
+ensures forall k :: 0 <= k < |lines| ==> lines[k].Length >= query.Length
+ensures forall k :: 0 <= k < |lines| ==> AnyMatch(lines[k], query)
 {
   var indexes;
-  found, indexes := GrepNaive(word, query);
+  var all := splitArrayBy(word, '\n');
+  var line := 0;
+  lines := [];
 
-  if !found {
-    rst := [];
-    return found, rst;
-  }
-
-  var wordSeq := word[..];
-  rst := [];
-  var i := 0;
-  while i < |indexes| 
-  
+  while line < all.Length 
+  invariant forall i :: 0 <= i < |lines| ==> lines[i].Length >= query.Length
+  invariant forall i :: 0 <= i < |lines| ==> AnyMatch(lines[i], query)
   {
-    var low, high := indexes[i], indexes[i] + query.Length;
-    rst := rst + "<-" + wordSeq[low..high] + "->";
-
-    low := high;
-    if i < |indexes| - 1 {
-      high := indexes[i + 1];
-    } else {
-      high := |wordSeq|;
+    var cur := all[line];
+    if cur.Length >= query.Length {
+      found, indexes := GrepNaive(cur, query);
+      if found {
+        assert forall k :: 0 <= k < |indexes| ==> IndexIsMatch(cur, query, indexes[k]);
+        lines := lines + [cur];
+      }
     }
-      // substituir isto pelo sorted
-    if low < high {
-      rst := rst + wordSeq[low..high];//"...";
-    }
-    
-    i := i + 1;
+    line := line + 1;
   }
-
-
+ 
 }
 
 method {:main} Main(ghost env:HostEnvironment?)
@@ -210,19 +277,15 @@ method {:main} Main(ghost env:HostEnvironment?)
       return;
     }
   
-    //var found, pos:= Grep(word, query);
-
-
-    //if found {
-    // print "YES",", ", pos;
-    //}
-    //else {
-    //  print "NO";
-    //}
     var found, rst := BashGrep(word, query);
 
     if found {
-      print rst;
+      print "Matching lines\n";
+      var l := 0;
+      while l < |rst| {
+        print rst[l][..]; 
+        l := l + 1;
+      }
     }
 
 }
